src/dvspec/dafny/specification/consensus.dfy
@@ -156,4 +156,6 @@ module ConsensusSpec
         )
      
     }    
+
+    
 }
